certicoq/theories/common/ExtLibMisc.v
@@ -6,19 +6,4 @@ Require Import Coq.Lists.List.
 Import ListNotations.
 
 
-Definition flatten {m} {A: Type} `{Monad m} (lm:list (m A)) : m (list A) :=
-fold_right (fun a l => l <- l;; 
-                       a <- a;; 
-                      ret (a :: l))
-          (ret []) 
-          lm.
-
-
-Require Import ExtLib.Data.Monads.OptionMonad.
-
-(*
-Eval vm_compute in flatten ([Some 1; Some 2]).
-Some [1; 2]
-
-fold_left results in a reverse order.
-*)
+(* the content from here moved to SquiggleEq.ExtLibMisc. *)
